src/prop/PFConsistent.v
@@ -1,0 +1,53 @@
+Require Import Omega.
+Require Import RelationClasses.
+
+Require Import sflib.
+Require Import paco.
+
+Require Import Axioms.
+Require Import Basic.
+Require Import DataStructure.
+Require Import DenseOrder.
+Require Import Event.
+Require Import Time.
+Require Import Language.
+Require Import View.
+Require Import Cell.
+Require Import Memory.
+Require Import TView.
+Require Import Thread.
+
+Require Import SimMemory.
+Require Import SimPromises.
+Require Import SimLocal.
+Require Import FulfillStep.
+Require Import MemoryReorder.
+
+Require Import SmallStep.
+Require Import PromiseConsistent.
+Require Import ReorderPromises.
+
+Set Implicit Arguments.
+
+
+Definition pf_consistent lang (e:Thread.t lang): Prop :=
+  forall sc1 mem1
+    (FUTURE: Memory.future e.(Thread.memory) mem1)
+    (FUTURE: TimeMap.le e.(Thread.sc) sc1)
+    (WF: Local.wf e.(Thread.local) mem1)
+    (SC: Memory.closed_timemap sc1 mem1)
+    (MEM: Memory.closed mem1),
+  exists e2,
+    <<STEPS: rtc (@Thread.tau_program_step lang) (Thread.mk lang e.(Thread.state) e.(Thread.local) sc1 mem1) e2>> /\
+    <<PROMISES: e2.(Thread.local).(Local.promises) = Memory.bot>>.
+
+Lemma consistent_pf_consistent:
+  Thread.consistent <2= pf_consistent.
+Proof.
+  s. ii. exploit PR; eauto. i. des.
+  exploit tau_steps_pf_tau_steps; eauto.
+  { ii. rewrite PROMISES, Memory.bot_get in *.  congr. }
+  i. des.
+  exploit rtc_promise_step_evt_bot; eauto. i. subst.
+  esplits; eauto.
+Qed.
